src/PlutusIR/Semantics/SemanticEquivalence/Multisubstitution/Congruence.v
@@ -1,5 +1,6 @@
 Require Import PlutusCert.PlutusIR.Semantics.Dynamic.
 Require Import PlutusCert.PlutusIR.Semantics.Static.
+Require Import PlutusCert.PlutusIR.Semantics.SemanticEquivalence.LogicalRelation.
 Require Import PlutusCert.Util.
 Require Import PlutusCert.Util.List.
 Require Import PlutusCert.Util.Map.
@@ -289,6 +290,12 @@ Proof.
 (* ADMIT: I had no time to finish this. Should hold, it is a congruence lemma. *)
 Admitted.
 
+Lemma msubstA_LetRec : forall ss bs e,
+    msubstA_term ss (Let Rec bs e) = Let Rec (msubstA_bindings_rec (mdrop (btvbs bs) ss) bs) (msubstA_term (mdrop (btvbs bs) ss) e).
+Proof.
+(* ADMIT: I had no time to finish this. Should hold, it is a congruence lemma. *)
+Admitted.
+
 Lemma msubstA_TermBind : forall ss stricty x T e,
     msubstA_binding ss (TermBind stricty (VarDecl x T) e) = TermBind stricty (VarDecl x (msubstT ss T)) (msubstA_term ss e).
 Proof.
@@ -310,3 +317,249 @@ Proof. induction ss; intros; auto. Qed.
 Lemma msubst_bindings_nonrec__fold : forall ss x v bs,
     msubst_bindings_nonrec ss <{ [v / x][bnr] bs }> = msubst_bindings_nonrec ((x, v) :: ss) bs.
 Proof. induction ss; intros; auto. Qed.
+
+Lemma msubst_LamAbs : forall ss x T t0,
+    msubst_term ss (LamAbs x T t0) = LamAbs x T (msubst_term (drop x ss) t0).
+Proof.
+  induction ss; intros.
+  - reflexivity.
+  - destruct a.
+    simpl.
+    destruct (s =? x)%string eqn:Heqb.
+    + eauto using eqb_eq.
+    + eauto using eqb_neq.
+Qed.
+
+Lemma msubstA_LamAbs : forall ss x T t0,
+    msubstA_term ss (LamAbs x T t0) = LamAbs x (msubstT ss T) (msubstA_term ss t0).
+Proof.
+  induction ss; intros.
+  - reflexivity.
+  - destruct a. eauto.
+Qed.
+
+Lemma msubstT_TyFun : forall ss T1 T2,
+    msubstT ss (Ty_Fun T1 T2) = Ty_Fun (msubstT ss T1) (msubstT ss T2).
+Proof.
+  induction ss.
+  - reflexivity.
+  - destruct a. eauto.
+Qed.
+
+Lemma msubst_Apply : forall ss t1 t2,
+    msubst_term ss (Apply t1 t2) = Apply (msubst_term ss t1) (msubst_term ss t2).
+Proof.
+  induction ss; intros.
+  - reflexivity.
+  - destruct a. eauto.
+Qed.
+
+Lemma msubstA_Apply : forall ss t1 t2,
+    msubstA_term ss (Apply t1 t2) = Apply (msubstA_term ss t1) (msubstA_term ss t2).
+Proof.
+  induction ss; intros.
+  - reflexivity.
+  - destruct a. eauto.
+Qed.
+
+Lemma msubst_Builtin : forall ss f,
+    msubst_term ss (Builtin f) = Builtin f.
+Proof. 
+  induction ss; intros.
+  - reflexivity.
+  - destruct a. eauto.
+Qed.
+
+Lemma msubstA_Builtin : forall ss f,
+    msubstA_term ss (Builtin f) = Builtin f.
+Proof. 
+  induction ss; intros.
+  - reflexivity.
+  - destruct a. eauto.
+Qed.
+
+Lemma msubst_Constant : forall ss sv,
+    msubst_term ss (Constant sv) = Constant sv.
+Proof.
+  induction ss; intros. 
+  - reflexivity.
+  - destruct a.
+    eauto.
+Qed.
+
+Lemma msubstA_Constant : forall ss sv ,
+    msubstA_term ss (Constant sv) = Constant sv.
+Proof.
+  induction ss; intros. 
+  - reflexivity.
+  - destruct a. eauto.
+Qed.
+
+Lemma msubstT_TyBuiltin : forall ss u,
+    msubstT ss (Ty_Builtin (Some (TypeIn u))) = Ty_Builtin (Some (TypeIn u)).
+Proof.
+  induction ss; intros.
+  - reflexivity.
+  - destruct a. eauto.
+Qed.
+
+Lemma msubst_DatatypeBind : forall ss X YKs matchFunc cs,
+    msubst_binding ss (DatatypeBind (Datatype X YKs matchFunc cs)) = DatatypeBind (Datatype X YKs matchFunc cs).
+Proof.
+  induction ss; intros.
+  - reflexivity.
+  - destruct a. eauto.
+Qed.
+
+Lemma msubstA_DatatypeBind : forall ss X YKs matchFunc cs,
+    msubstA_binding ss (DatatypeBind (Datatype X YKs matchFunc cs)) = DatatypeBind (Datatype X YKs matchFunc (msubstA_constructors ss cs)).
+Proof.
+  induction ss; intros.
+  - reflexivity.
+  - destruct a. simpl. eauto.
+Qed.
+
+
+Lemma msubst_Error : forall ss T,
+    msubst_term ss (Error T) = Error T.
+Proof. 
+  induction ss; intros.
+  - reflexivity.
+  - destruct a. eauto.
+Qed.
+
+Lemma msubstA_Error : forall ss T,
+    msubstA_term ss (Error T) = Error (msubstT ss T).
+Proof.
+  induction ss; intros.
+  - reflexivity.
+  - destruct a. eauto.
+Qed.
+
+Lemma msubst_IWrap : forall ss F T M,
+    msubst_term ss (IWrap F T M) = IWrap F T (msubst_term ss M).
+Proof. 
+  induction ss; intros.
+  - reflexivity.
+  - destruct a. eauto.
+Qed. 
+
+Lemma msubstA_IWrap : forall ss F T M,
+    msubstA_term ss (IWrap F T M) = IWrap (msubstT ss F) (msubstT ss T) (msubstA_term ss M).
+Proof.
+  induction ss; intros.
+  - reflexivity.
+  - destruct a. eauto.
+Qed. 
+
+Lemma msubstT_IFix : forall ss F T,
+    msubstT ss (Ty_IFix F T) = Ty_IFix (msubstT ss F) (msubstT ss T).
+Proof.
+  induction ss; intros.
+    - reflexivity.
+    - destruct a. eauto.
+Qed. 
+
+Lemma msubst_TyAbs : forall ss bX K t0,
+    msubst_term ss (TyAbs bX K t0) = TyAbs bX K (msubst_term ss t0).
+Proof. induction ss; intros. - reflexivity. - destruct a. eauto. Qed.
+
+Lemma msubstA_TyAbs : forall ss bX K t0,
+    msubstA_term ss (TyAbs bX K t0) = TyAbs bX K (msubstA_term (drop bX ss) t0).
+Proof. induction ss; intros. - reflexivity. - intros. destruct a. simpl. destruct (s =? bX)%string; eauto. Qed.
+
+
+Lemma msubstT_TyForall : forall ss bX K T,
+    msubstT ss (Ty_Forall bX K T) = Ty_Forall bX K (msubstT (drop bX ss) T).
+Proof. induction ss; intros. - reflexivity. - intros. destruct a. simpl. destruct (s =? bX)%string; eauto. Qed.
+
+Lemma msubst_TyInst : forall ss t0 T0,
+    msubst_term ss (TyInst t0 T0) = TyInst (msubst_term ss t0) T0.
+Proof. induction ss; intros. - reflexivity. - destruct a. eauto. Qed.
+
+
+Lemma msubstA_TyInst : forall ss t0 T0,
+    msubstA_term ss (TyInst t0 T0) = TyInst (msubstA_term ss t0) (msubstT ss T0).
+Proof. induction ss; intros. - reflexivity. - destruct a. eauto. Qed.
+
+
+Lemma msubst_Unwrap : forall ss M,
+    msubst_term ss (Unwrap M) = Unwrap (msubst_term ss M).
+Proof. induction ss; intros. - reflexivity. - destruct a. eauto. Qed.
+
+Lemma msubstA_Unwrap : forall ss M ,
+    msubstA_term ss (Unwrap M) = Unwrap (msubstA_term ss M).
+Proof. induction ss; intros. - reflexivity. - destruct a. eauto. Qed.
+
+
+Lemma msubst_Var : forall ss x,
+    closed_env ss ->
+    msubst_term ss (Var x) =
+      match lookup x ss with
+      | Datatypes.Some t => t
+      | None => Var x
+      end.
+Proof. 
+  induction ss; intros. 
+  - reflexivity. 
+  - intros. 
+    destruct a. 
+    simpl. 
+    destruct (s =? x)%string eqn:Heqb.
+    + apply eqb_eq in Heqb as Heq.
+      subst.
+      destruct H.
+      rewrite msubst_closed.
+      all: auto.
+    + apply eqb_neq in Heqb as Hneq.
+      destruct H.
+      eapply IHss.
+      assumption.
+Qed.
+
+Lemma msubstA_Var : forall ss x,
+    msubstA_term ss (Var x) = Var x.
+Proof. induction ss; intros. - reflexivity. - destruct a. eauto. Qed.
+
+
+(* TODO move this into separate module*)
+
+Hint Rewrite
+  msubstA_LetRec
+  msubstA_LetNonRec
+  msubstA_bnr__bvbs
+  msubstA_LetNonRec_nil
+  msubstA_LetNonRec
+  msubstA_LetRec
+  msubstA_TermBind
+  msubstA_BindingsNonRec_cons
+  msubstA_LamAbs
+  msubstA_Apply
+  msubstA_Builtin
+  msubstA_Constant
+  msubstA_DatatypeBind
+  msubstA_Error
+  msubstA_IWrap
+  msubstA_TyAbs
+  msubstA_TyInst
+  msubstA_Unwrap
+  msubstA_Var
+  : msubstA_cong.
+
+Lemma not_is_error_msubstA : forall v ss, ~ is_error v -> ~ is_error (msubstA_term ss v).
+  intros v ss H_not_err H_err.
+  destruct v; simpl in H_err.
+  all: try (autorewrite with msubstA_cong in H_err; inversion H_err).
+
+  (* Let r bs t *)
+  - destruct r.
+    + autorewrite with msubstA_cong in H_err.
+       inversion H_err.
+    + rewrite msubstA_LetRec in H_err.
+       inversion H_err.
+
+  (* Error *)
+  - apply H_not_err.
+    constructor.
+Qed.
+
